Add more BNA lemmas, and better sort things

nondeterministic_dataflow/BNA_Operators.thy
@@ -1,13 +1,480 @@
-section \<open>The BNA operators operator\<close>
-
+section \<open>The BNA operators\<close>
+\<comment> \<open>The basic operators - except compositions, loop and fair merge- from the BNA book "Network Algebra for Synchronous and Asynchronous Dataflow" (https://staff.fnwi.uva.nl/c.a.middelburg/papers/P9508.pdf) \<close>
+\<comment> \<open>Here we list most of the axioms from Table 1, and Table 4\<close>
 theory BNA_Operators
 
 imports
   Operator
-  Loop
-  Composition
+  Composition_Choices
 begin
+section \<open>spin_op/end_op/I_0\<close>
+abbreviation end_op ("\<oslash>") where "end_op \<equiv> Choice cempty"
+\<comment> \<open>spin_op/end_op is I_0 in the BNA book\<close>
+\<comment> \<open>In the transition system this is a dead-lock\<close>
 
+\<comment> \<open>Some useful functions for defining operators\<close>
+abbreviation "safe_choice_stop stop f ops \<equiv> (if ops = cempty then stop else Choice (cimage f ops))"
+abbreviation "safe_choice f \<equiv> safe_choice_stop (f end_op) f"
+abbreviation "safe_choice2 f op1s op2s \<equiv> (if op1s = cempty \<and> op2s = cempty then end_op
+  else if op1s = cempty then Choice (cimage (f end_op) op2s)
+  else if op2s = cempty then Choice (cimage (\<lambda>op1. f op1 end_op) op1s)
+  else Choice (cimage (case_prod f) (cproduct op1s op2s)))"
+abbreviation "choice1 op \<equiv> Choice (cimage (\<lambda>_. op) {|()|})"
+abbreviation "choice2 op1 op2 \<equiv> Choice (cimage (\<lambda>b. if b then op1 else op2) (cinsert True (csingle False)))"
+abbreviation "safe_read f x \<equiv> (case x of None \<Rightarrow> end_op | Some x \<Rightarrow> f x)"
+
+corec spin_op :: "('a, 'b, 'd) op" ("\<otimes>") where
+  "spin_op = Choice (cimage (\<lambda> _. spin_op) (csingle ()))"
+
+abbreviation "ARead i f op \<equiv> Choice (cimage (\<lambda> x. if x then op else Read i f) (cinsert True (csingle False)))"
+lemma ARead_simp[simp]: "ARead i f op = Choice ({| op, Read i f |})"
+  by simp
+
+lemma finished_spin_op[simp]:
+  "finished \<otimes>"
+  apply coinduction
+  apply (subst spin_op.code)
+  apply auto
+  done
+
+lemma finished_end_op[simp]:
+  "finished \<oslash>"
+  by coinduction blast
+
+lemma step_end_op[simp]: "step l \<oslash> t' = False"
+  by auto
+
+lemma spin_op_finished[simp]:
+  "finished \<otimes>"
+  apply coinduction
+  apply (subst spin_op.code)
+  apply (auto 0 0 simp add:  sup_cset.rep_eq cinsert.rep_eq cimage.rep_eq bot_cset.rep_eq; hypsubst_thin?)
+  done
+
+lemma choices_spin_op[simp]:
+  "choices \<otimes> = {||}"
+  by (simp add: finished_choices_empty)
+
+lemma traces_end_op[simp]:
+  "traces \<oslash> = {LNil}"
+  by (auto simp: traces_def intro: finished.intros traced.intros step.intros elim: traced.cases)
+
+lemma step_spin_op_no_label:
+  "step io \<otimes> op \<Longrightarrow> False"
+  using spin_op_finished step_not_finished by blast
+
+lemma
+  "(spin_op \<parallel> spin_op) ~ spin_op"
+  apply (coinduction rule: bisim_coinduct_upto)
+  apply safe
+  subgoal
+    unfolding pcomp_op_def sim_def
+    apply auto
+    apply (subst (asm) comp_op_code)
+    apply auto
+    done
+  subgoal
+    unfolding pcomp_op_def sim_def
+    apply auto
+    using step_spin_op_no_label apply blast
+    done
+  done
+
+\<comment> \<open>TODO: both are delta\<close>
+lemma "\<otimes> ~ \<oslash>"
+  oops
+
+section \<open>id_op/\<I>/I_m\<close>
+\<comment> \<open>id_op is I_m in the BNA paper\<close>
+
+datatype (discs_sels) ('m, 'd) id_op_aux =
+  id_Read_aux "'m" "'d \<Rightarrow> ('m \<Rightarrow> 'd buf)"
+  | id_Write_aux "('m \<Rightarrow> 'd buf)" "'m" 'd 
+  | id_Silent_aux "('m \<Rightarrow> 'd buf)"
+
+abbreviation eval_id_op_aux where
+  "eval_id_op_aux c aux \<equiv> (case aux of
+    id_Read_aux p f \<Rightarrow> Read p (\<lambda>y. let buf = f y in c buf)
+  | id_Write_aux buf q x \<Rightarrow> (Write (c buf) q x))"
+
+corec id_op :: "_ \<Rightarrow> ('m :: countable, 'm, 'd) op" where
+  "id_op buf = Choice (cimage (eval_id_op_aux id_op) (cUn 
+    (cimage (\<lambda> p. id_Read_aux p (\<lambda> x. BENQ p x buf)) (cUNIV :: 'm cset)) 
+    (cimage (\<lambda> p. id_Write_aux (BTL p buf) p (BHD p buf)) (cfilter (\<lambda> p. buf p \<noteq> []) (cUNIV :: 'm cset)))))"
+
+abbreviation id_empty_op ("\<I>") where
+  "\<I> \<equiv> id_op (\<lambda> _. [])"
+
+lemma id_op_code:
+  "id_op buf = Choice (cUn 
+    (cimage (\<lambda> p. Read p ((\<lambda> x. id_op (BENQ p x buf)))) (cUNIV :: 'm cset))
+    (cimage (\<lambda> p. Write (id_op (BTL p buf)) p  (BHD p buf)) (cfilter (\<lambda> p. buf p \<noteq> []) (cUNIV :: ('m :: countable) cset))))"
+  apply (subst id_op.code)
+  apply (unfold cimage_cUn cimage_cinsert op.inject)
+  apply simp
+  apply (rule arg_cong2[where f = cUn])
+   apply (auto simp add: cset.map_comp o_def cimage_cUn intro!: arg_cong2[where f = cUn] cimage_cong
+      split: id_op_aux.splits op.splits option.splits)
+  done
+
+subsection \<open>Some basic properties id_op\<close>
+lemma step_id_op_Inp:
+  "step io (id_op buf) op' \<Longrightarrow>
+   io = Inp p x \<Longrightarrow>
+   op' = id_op (BENQ p x buf)"
+  apply (induct io "id_op buf" op' arbitrary: buf rule: step.induct)
+    apply simp_all
+   apply (subst (asm) id_op_code)
+   apply simp
+  apply (subst (asm) (3) id_op_code)
+  apply auto
+  done
+
+lemma step_id_op_Out:
+  "step io (id_op buf) op' \<Longrightarrow>
+   io = Out p x \<Longrightarrow>
+   op' = id_op (BTL p buf) \<and> BHD p buf = x \<and> buf p \<noteq> []"
+  apply (induct io "id_op buf" op' arbitrary: buf rule: step.induct)
+    apply simp_all
+   apply (subst (asm) id_op_code)
+  apply simp
+  apply (subst (asm) (3) id_op_code)
+  apply auto
+  done
+
+lemma choices_id_op[simp]:
+  "choices (id_op buf) = cUn (cUnion (cimage choices (cimage (\<lambda>p. Read p (\<lambda>x. id_op (buf(p := bulk_benq [x] (buf p))))) cUNIV)))
+       (cUnion (cimage choices (cimage (\<lambda>p. Write (id_op (buf(p := btl (buf p)))) p (BHD p buf)) (cfilter (\<lambda>p. buf p \<noteq> []) cUNIV))))"
+  apply (subst id_op_code)
+  apply simp
+  done
+
+subsection \<open>Compositional properties id_op\<close>
+lemma step_comp_op_Some_id_op_id_op:
+  "step io (comp_op Some buf2 op1 op2) op \<Longrightarrow>
+   op1 = id_op buf1 \<Longrightarrow>
+   op2 = id_op buf3 \<Longrightarrow>
+   (\<exists> p x. io = Inp (Inl p) x \<and>
+     (\<exists> buf1' buf2' buf3'. op = comp_op Some buf2' (id_op (BENQ p x buf1')) (id_op buf3') \<and>
+      buf1 >> buf2 >> buf3 = buf1' >> buf2' >> buf3')) \<or>
+
+   (\<exists> p x. io = Out (Inr p) x \<and>
+     (\<exists> buf1' buf2' buf3'. op = comp_op Some buf2' (id_op buf1') (id_op (BTL p buf3')) \<and> BHD p buf3' = x \<and> buf3' p \<noteq> [] \<and>
+     buf1 >> buf2 >> buf3 = buf1' >> buf2' >> buf3')) \<or>
+
+   (\<exists> p x. io = Tau \<and>
+     (\<exists> buf1' buf2' buf3'. op = comp_op Some (BTL p buf2') (id_op buf1') (id_op (BENQ p x buf3')) \<and> BHD p buf2' = x \<and> buf2' p \<noteq> [] \<and>
+     buf1 >> buf2 >> buf3 = buf1' >> buf2' >> buf3')) \<or>
+
+   (\<exists> p x. io = Tau \<and>
+     (\<exists> buf1' buf2' buf3'. op = comp_op Some (BENQ p x buf2') (id_op (BTL p buf1')) (id_op buf3') \<and> BHD p buf1' = x \<and> buf1' p \<noteq> [] \<and>
+     buf1 >> buf2 >> buf3 = buf1' >> buf2' >> buf3'))"
+  apply (induction io "comp_op Some buf2 op1 op2" op arbitrary: op1 op2 buf1 buf2 buf3 rule: step.induct)
+  subgoal
+    apply hypsubst_thin
+    apply (subst (asm) comp_op_code)
+    apply auto
+    done
+  subgoal
+    apply hypsubst_thin
+    apply (subst (asm) comp_op_code)
+    apply auto
+    done
+  subgoal
+    apply hypsubst_thin
+    apply (subst (asm) comp_op_code)
+    apply auto
+    done
+  subgoal for op ops io op' op1 op2 buf2 buf1 buf3
+    apply hypsubst_thin
+    apply (subst (asm) (6) comp_op_code)
+    apply (auto 0 0)
+                     apply blast+
+    done
+  done
+
+subsection \<open>Axiom: B4\<close>
+lemma id_id_gen:
+  "map_op projl projr (comp_op Some buf2 (id_op buf1) (id_op buf3)) \<approx> id_op (buf1 >> buf2 >> buf3)"
+  apply (coinduction arbitrary: buf1 buf2 buf3 rule: wbisim_coinduct_upto)
+  subgoal for buf1 buf2 buf3
+    unfolding wsim_def
+    apply auto
+    subgoal for io op
+      apply (drule step_map_op_inv)
+      apply safe
+      apply hypsubst_thin
+      subgoal for io' op'
+        apply (drule step_comp_op_Some_id_op_id_op)
+          apply (rule refl)+
+        apply simp
+        apply (elim disjE exE conjE)
+        subgoal for p x buf1' buf2' buf3'
+          apply hypsubst_thin
+          apply (intro conjI exI)
+           apply (subst id_op_code)
+          apply (rule step_wstep)
+           apply (rule SC[rotated])
+            apply simp
+            apply (rule SR)
+           apply simp
+           apply (rule disjI1)
+           apply (rule image_eqI)
+            apply (rule refl)
+           apply simp
+          apply (rule wbc_base)
+          apply (intro conjI exI)
+           apply (rule refl)
+          apply (rule arg_cong[where f=id_op])
+          apply (rule ext)
+          apply simp
+          apply metis
+          done
+        subgoal for p x buf1' buf2' buf3'
+          apply hypsubst_thin
+          apply simp
+          apply (intro conjI exI)
+           apply (subst id_op_code)
+          apply (rule step_wstep)
+           apply (rule SC[rotated])
+            apply (rule SW)
+           apply simp
+           apply (rule disjI2)
+           apply (rule image_eqI)
+            apply force
+           apply (simp add: cUNIV.rep_eq)
+          apply (rule wbc_base)
+          apply (intro conjI exI)
+           apply (rule refl)
+          apply (rule arg_cong[where f=id_op])
+          apply (rule ext)
+          apply simp
+          done
+        subgoal for p buf1' buf2' buf3'
+          apply hypsubst_thin
+          apply (intro conjI exI)
+           apply (subst id_op_code)
+          oops
+(* 
+          apply (rule step_step_tau_wstep[rotated])
+           apply (rule SC[rotated])
+            apply simp
+            apply (rule ST)
+           apply simp
+           apply (rule disjI1)
+           apply (rule refl)
+          apply (rule bc_base)
+          apply (intro conjI exI)
+           apply (rule refl)
+          apply (rule arg_cong[where f=id_op])
+          apply (rule ext)
+          apply simp
+          done
+        subgoal for p buf1' buf2' buf3'
+          apply hypsubst_thin
+          apply (intro conjI exI)
+           apply (subst id_op_code)
+           apply (rule SC[rotated])
+            apply simp
+            apply (rule ST)
+           apply simp
+           apply (rule disjI1)
+           apply (rule refl)
+          apply (rule bc_base)
+          apply (intro conjI exI)
+           apply (rule refl)
+          apply (rule arg_cong[where f=id_op])
+          apply (rule ext)
+          apply simp
+          done
+        done
+      done
+    subgoal for io op1'
+      apply (cases io)
+      subgoal for p x
+        apply hypsubst_thin
+        apply (drule step_id_op_Inp)
+         apply simp
+        apply hypsubst_thin
+        apply (rule exI[of _ "map_op projl projr (comp_op Some buf2 (id_op (BENQ p x buf1)) (id_op buf3))"])
+        apply (intro conjI)
+        subgoal
+          apply (rule step_map_op[where f=projl and g=projr and io="Inp (Inl p) x", simplified])
+           apply (subst comp_op_code)
+           apply simp
+           apply (rule SC)
+            apply (simp add: Set.filter_def)
+            apply (rule disjI2)
+            apply simp
+            apply (rule disjI1)
+            apply (rule image_eqI)
+             apply (rule refl)
+            apply simp
+            apply (rule disjI1)
+            apply (intro exI)
+            apply (rule refl)
+           apply simp_all
+          apply (rule SR)
+          done
+        subgoal
+          apply (rule bc_sym)
+          apply (rule bc_base)
+          apply (intro conjI exI)
+           apply simp_all
+          apply (rule arg_cong[where f=id_op])
+          apply auto
+          done
+        done
+      subgoal for p x
+        apply hypsubst_thin
+        apply (drule step_id_op_Out)
+         apply simp
+        apply (elim conjE)
+        apply (drule BHD_BAPPEND_2_cases)
+         apply simp
+        apply hypsubst_thin
+        apply (elim exE disjE conjE)
+        subgoal
+          apply (rule exI[of _ "map_op projl projr (comp_op Some buf2 (id_op buf1) (id_op (BTL p buf3)))"])
+          apply (intro conjI)
+          subgoal
+            apply (rule step_map_op[where f=projl and g=projr and io="Out (Inr p) x", simplified])
+             apply (subst comp_op_code)
+             apply simp
+             apply (rule SC)
+              apply (simp add: Set.filter_def)
+              apply (rule disjI2)
+              apply simp
+              apply (rule disjI2)
+              apply (rule image_eqI)
+               apply (rule refl)
+              apply (simp add: cUNIV.rep_eq)
+              apply (intro conjI)
+               apply (rule disjI2)
+               apply (rule disjI2)
+               apply (intro conjI exI)
+                apply assumption
+               apply (rule refl)
+              apply (auto simp add: step.intros(2))
+            done
+          subgoal
+            apply (rule bc_sym)
+            apply (rule bc_base)
+            apply (intro exI conjI) 
+             apply (rule refl)
+            apply (rule arg_cong[where f=id_op])
+            apply (rule ext)
+            apply (auto simp only: split: if_splits)
+              apply (smt (verit, best) fun_upd_apply tl_append2)+
+            done
+          done
+        subgoal
+          apply (rule exI[of _ "map_op projl projr (comp_op Some (BTL p buf2) (id_op buf1) (id_op buf3))"])
+          apply (intro conjI)
+          subgoal
+            apply (rule step_map_op[where f=projl and g=projr and io="Out (Inr p) x", simplified])
+            apply (subst comp_op_code)
+            apply simp
+            apply (rule SC)
+             apply simp
+             apply (rule disjI2)+
+             apply (rule image_eqI)
+              apply (rule refl)
+             apply (simp add: Set.filter_def cUNIV.rep_eq)
+              apply (intro conjI)
+               apply (rule disjI2)
+               apply (rule disjI1)
+            apply (intro conjI exI)
+               apply simp_all
+             apply force
+            apply simp *)
+
+\<comment> \<open>TODO: id o id is id\<close>
+subsubsection \<open>Axiom: B4\<close>
+lemma scomp_op_id_id:
+  "\<I> \<bullet> \<I> \<approx> \<I>"
+  unfolding scomp_op_def
+ (*  using id_id_gen[of "\<lambda> _. []" "\<lambda> _. []" "\<lambda> _. []"] apply simp
+  done *)
+  oops
+
+subsection \<open>Axiom: B6\<close>
+subsubsection \<open>Auxiliary lemmas\<close>
+subsubsection \<open>Axiom: B6\<close>
+lemma pcomp_op_id_id:
+  "\<I> \<parallel> \<I> ~ \<I>"
+  oops
+
+section \<open>dummy_source_op\<close>                                     
+abbreviation dummy_source_op ("\<exclamdown>") where
+  "\<exclamdown> \<equiv> \<oslash> \<bullet> \<I>"
+
+subsection \<open>Axiom: A12\<close>
+lemma dummy_source_op_end_op:
+ "\<exclamdown> ~ \<oslash>"
+  oops
+lemma dummy_source_op_spin_op:
+ "\<exclamdown> = \<otimes>"
+  oops
+
+subsection \<open>Axiom: A13\<close>
+lemma pcomp_opdummy_source:
+ "\<exclamdown> \<parallel> \<exclamdown> ~ \<exclamdown>"
+  oops
+
+section \<open>sink_op\<close>                                     
+corec drain_op :: "('m :: countable, 'o, 'd) op" where
+  "drain_op = Choice ((cimage (\<lambda> p. Read p (\<lambda> x. drain_op)) (cUNIV :: 'm cset)))"
+
+abbreviation "sink_gen_op buf \<equiv> id_op (\<lambda> _. []) \<bullet> drain_op"
+abbreviation sink_op ("!") where
+  "! \<equiv> \<I> \<bullet> drain_op"
+abbreviation "sink_0_op \<equiv> \<oslash>"
+
+subsection \<open>Axiom: A16\<close>
+lemma
+  "sink_0_op = \<oslash>"
+  by simp
+
+subsection \<open>Axiom: A9\<close>
+lemma
+  "\<exclamdown> \<bullet> sink_0_op ~ \<oslash>"
+  oops
+lemma
+  "\<exclamdown> \<bullet> ! = \<otimes>"
+  oops
+
+
+end
+corec sink_op :: "('a, 'b, 'd) op" where
+  "sink_op = Read 1 (\<lambda>_. sink_op)"
+
+lemma choices_sink_op[simp]:
+  "choices sink_op = {|Read 1 (\<lambda> _. sink_op)|}"
+  unfolding choices_def
+  apply safe
+  subgoal premises prems for x n
+    using prems(2) apply -
+    apply (induct n)
+     apply (subst (asm) sink_op.code)
+     apply simp 
+    apply (subst (asm) (3) sink_op.code)
+    apply simp
+    done
+  subgoal for x
+    apply auto
+    apply (metis UNIV_witness natcUNIV.rep_eq choices_at.simps(1) cin.rep_eq cinsertI1 sink_op.code)
+    done
+  done
+
+section \<open>transp_op - transposition operator\<close>
+\<comment> \<open>TODO: define the operator + write and prove axioms B7, B8, B9, B10, R1, F2, \<close>
+
+section \<open>User defined operators\<close>
+abbreviation buffered ("\<stileturn> _ \<turnstile>" [150]151) where
+  "\<stileturn>op\<turnstile> \<equiv> \<I> \<bullet> op \<bullet> \<I>"
+
+(* 
 abbreviation "write op p x \<equiv> Write op p (Observed x)"
 abbreviation "eob op p \<equiv> Write op p EOB"
 abbreviation "eos op p \<equiv> Write op p EOS"
@@ -41,5 +508,5 @@ lemma
   using assms unfolding history_def traced_pcomp_op'
   apply auto
   oops
- 
+  *)
 end
