nondeterministic_dataflow/Composition_Choices.thy
@@ -7,13 +7,13 @@ imports
 begin
 
 (*workaround about termination issue in corecursive*)
-lemma case_prod_cong4[fundef_cong]:
+(* lemma case_prod_cong4[fundef_cong]:
   fixes prod prod' f g
   shows "prod = prod' \<Longrightarrow>
     (\<And>x1 x2 y1 y2. prod' = ((x1, x2), (y1, y2)) \<Longrightarrow> f x1 x2 y1 y2 = g x1 x2 y1 y2) \<Longrightarrow>
     ((\<lambda>((x1, x2), (y1, y2)). f x1 x2 y1 y2) prod) = ((\<lambda>((x1, x2), (y1, y2)). g x1 x2 y1 y2) prod')"
   by (auto split: prod.splits)
-
+ *)
 datatype (discs_sels) ('ip1, 'ip2, 'op1, 'op2, 'd) comp_op_aux =
   Read_aux "'ip1 + 'ip2" "'d \<Rightarrow> ('ip2 \<Rightarrow> 'd buf) \<times> ('ip1, 'op1, 'd) op \<times> ('ip2, 'op2, 'd) op"
   | Write_aux "('ip2 \<Rightarrow> 'd buf) \<times> ('ip1, 'op1, 'd) op \<times> ('ip2, 'op2, 'd) op" "'op1 + 'op2" 'd
@@ -118,66 +118,7 @@ lemma comp_op_simps[simp]:
           (sound_reads wire buf (cUnion (cimage choices op2s)))))" 
   by (subst comp_op_code, auto simp add: image_iff split: option.splits)+
 
-no_notation Sublist.parallel (infixl "\<parallel>" 50)
-
-definition pcomp_op (infixl "\<parallel>" 64) where
-  "pcomp_op = comp_op (\<lambda>_. None) (\<lambda>_. [])"
-
-definition scomp_op (infixl "\<bullet>" 65) where
-  "scomp_op op1 op2 = map_op projl projr (comp_op Some (\<lambda>_. []) op1 op2)"
-
-abbreviation id_empty_op ("\<I>") where
-  "\<I> \<equiv> id_op (\<lambda> _. [])"
-
-abbreviation buffered ("\<stileturn> _ \<turnstile>" [150]151) where
-  "\<stileturn>op\<turnstile> \<equiv> \<I> \<bullet> op \<bullet> \<I>"
-
-fun reassoc where
-  "reassoc (Inl (Inl x)) = Inl x"
-| "reassoc (Inl (Inr x)) = Inr (Inl x)"
-| "reassoc (Inr x) = Inr (Inr x)"
-
-fun assoc where
-  "assoc (Inl x) = Inl (Inl x)"
-| "assoc (Inr (Inl x)) = Inl (Inr x)"
-| "assoc (Inr (Inr x)) = Inr x"
-
-lemma reassoc_assoc[simp]:
-  "reassoc o assoc = id"
-  unfolding comp_def
-  apply (rule ext)
-  subgoal for x
-    apply (induct x rule: assoc.induct)
-      apply auto
-    done
-  done
-
-lemma assoc_reassoc[simp]:
-  "assoc o reassoc = id"
-  unfolding comp_def
-  apply (rule ext)
-  subgoal for x
-    apply (induct x rule: reassoc.induct)
-      apply auto
-    done
-  done
-
-lemma
-  "(spin_op \<parallel> spin_op) ~ spin_op"
-  apply (coinduction rule: bisim_coinduct_upto)
-  apply safe
-  subgoal
-    unfolding pcomp_op_def sim_def
-    apply auto
-    apply (subst (asm) comp_op_code)
-    apply auto
-    done
-  subgoal
-    unfolding pcomp_op_def sim_def
-    apply auto
-    using step_spin_op_no_label apply blast
-    done
-  done
+section \<open>Properties of the (general) composition\<close>
 
 lemma step_comp_op_L:
   "step io op1 op1' \<Longrightarrow>
@@ -313,19 +254,53 @@ lemma step_comp_op_R:
     done
   done
 
+section \<open>Parallel composition operator\<close>
+no_notation Sublist.parallel (infixl "\<parallel>" 50)
+
+definition pcomp_op (infixl "\<parallel>" 64) where
+  "pcomp_op = comp_op (\<lambda>_. None) (\<lambda>_. [])"
+
+fun reassoc where
+  "reassoc (Inl (Inl x)) = Inl x"
+| "reassoc (Inl (Inr x)) = Inr (Inl x)"
+| "reassoc (Inr x) = Inr (Inr x)"
+
+fun assoc where
+  "assoc (Inl x) = Inl (Inl x)"
+| "assoc (Inr (Inl x)) = Inl (Inr x)"
+| "assoc (Inr (Inr x)) = Inr x"
+
+lemma reassoc_assoc[simp]:
+  "reassoc o assoc = id"
+  unfolding comp_def
+  apply (rule ext)
+  subgoal for x
+    apply (induct x rule: assoc.induct)
+      apply auto
+    done
+  done
+
+lemma assoc_reassoc[simp]:
+  "assoc o reassoc = id"
+  unfolding comp_def
+  apply (rule ext)
+  subgoal for x
+    apply (induct x rule: reassoc.induct)
+      apply auto
+    done
+  done
+
+section \<open>Sequential composition operator\<close>
+definition scomp_op (infixl "\<bullet>" 65) where
+  "scomp_op op1 op2 = map_op projl projr (comp_op Some (\<lambda>_. []) op1 op2)"
+(* 
 abbreviation "read_or_write \<equiv> Choice {| Read (1::2) (\<lambda> _. end_op), Write (Read (2::2) (\<lambda> _. end_op)) (1::1) (1::nat) |}"
 
 lemma choices_read_or_write[simp]:
   "choices read_or_write = {| Read (1::2) (\<lambda> _. end_op), Write (Read (2::2) (\<lambda> _. end_op)) (1::1) (1::nat) |}"
   by (auto simp del: cimage_cinsert)
 
-lemma cUnion_cinsert[simp]:
-  "cUnion (cinsert x A) = cUn x (cUnion A)"
-  apply (subst (3 8) cset.map_id[symmetric])
-  apply fastforce
-  done
-
-lemma
+lemma assoc_example_1:
   "read_or_write \<bullet> ((end_op :: (1, 1, nat) op) \<bullet> (Write end_op (1::1) 1)) ~ read_or_write \<bullet> (end_op :: (1, 1, nat) op) \<bullet> (Write end_op (1::1) 1)"
   apply (coinduction rule: bisim_coinduct_upto)
   unfolding sim_def scomp_op_def
@@ -409,501 +384,6 @@ lemma
     subgoal
       using bisim_coinduct_upto by (force intro: step_map_op step.intros bc_refl)
     done
-  done
-
-lemma choices_id_op[simp]:
-  "choices (id_op buf) = cinsert (Silent (id_op buf))
-     (cUn (cUnion (cimage choices (cimage (\<lambda>p. Read p (\<lambda>x. id_op (buf(p := bulk_benq [x] (buf p))))) cUNIV)))
-       (cUnion (cimage choices (cimage (\<lambda>p. Write (id_op (buf(p := btl (buf p)))) p (BHD p buf)) (cfilter (\<lambda>p. buf p \<noteq> []) cUNIV)))))"
-  apply (subst id_op_code)
-  apply simp
-  done
-
-lemma step_comp_op_Some_id_op_id_op:
-  "step io (comp_op Some buf2 op1 op2) op \<Longrightarrow>
-   op1 = id_op buf1 \<Longrightarrow>
-   op2 = id_op buf3 \<Longrightarrow>
-   (\<exists> p x. io = Inp (Inl p) x \<and>
-     (\<exists> buf1' buf2' buf3'. op = comp_op Some buf2' (id_op (BENQ p x buf1')) (id_op buf3') \<and>
-      buf1 >> buf2 >> buf3 = buf1' >> buf2' >> buf3')) \<or>
-
-   (\<exists> p x. io = Out (Inr p) x \<and>
-     (\<exists> buf1' buf2' buf3'. op = comp_op Some buf2' (id_op buf1') (id_op (BTL p buf3')) \<and> BHD p buf3' = x \<and> buf3' p \<noteq> [] \<and>
-     buf1 >> buf2 >> buf3 = buf1' >> buf2' >> buf3')) \<or>
-
-   (io = Tau \<and> op = comp_op Some buf2 op1 op2) \<or>
-   (\<exists> p x. io = Tau \<and>
-     (\<exists> buf1' buf2' buf3'. op = comp_op Some (BTL p buf2') (id_op buf1') (id_op (BENQ p x buf3')) \<and> BHD p buf2' = x \<and> buf2' p \<noteq> [] \<and>
-     buf1 >> buf2 >> buf3 = buf1' >> buf2' >> buf3')) \<or>
-
-   (\<exists> p x. io = Tau \<and>
-     (\<exists> buf1' buf2' buf3'. op = comp_op Some (BENQ p x buf2') (id_op (BTL p buf1')) (id_op buf3') \<and> BHD p buf1' = x \<and> buf1' p \<noteq> [] \<and>
-     buf1 >> buf2 >> buf3 = buf1' >> buf2' >> buf3'))"
-  apply (induction io "comp_op Some buf2 op1 op2" op arbitrary: op1 op2 buf1 buf2 buf3 rule: step.induct)
-  subgoal
-    apply hypsubst_thin
-    apply (subst (asm) comp_op_code)
-    apply auto
-    done
-  subgoal
-    apply hypsubst_thin
-    apply (subst (asm) comp_op_code)
-    apply auto
-    done
-  subgoal
-    apply hypsubst_thin
-    apply (subst (asm) comp_op_code)
-    apply auto
-    done
-  subgoal for op ops io op' op1 op2 buf2 buf1 buf3
-    apply hypsubst_thin
-    apply (subst (asm) (7) comp_op_code)
-    apply (auto 0 0)
-                     apply blast+
-    done
-  done
-
-lemma id_id_gen:
-  "map_op projl projr (comp_op Some buf2 (id_op buf1) (id_op buf3)) ~ id_op (buf1 >> buf2 >> buf3)"
-  apply (coinduction arbitrary: buf1 buf2 buf3 rule: bisim_coinduct_upto)
-  subgoal for buf1 buf2 buf3
-    unfolding sim_def
-    apply auto
-    subgoal for io op
-      apply (drule step_map_op_inv)
-      apply safe
-      apply hypsubst_thin
-      subgoal for io' op'
-        apply (drule step_comp_op_Some_id_op_id_op)
-          apply (rule refl)+
-        apply simp
-        apply (elim disjE exE conjE)
-        subgoal for p x buf1' buf2' buf3'
-          apply hypsubst_thin
-          apply (intro conjI exI)
-           apply (subst id_op_code)
-           apply (rule SC[rotated])
-            apply simp
-            apply (rule SR)
-           apply (rule cinsertI2)
-           apply simp
-           apply (rule disjI1)
-           apply (rule image_eqI)
-            apply (rule refl)
-           apply simp
-          apply (rule bc_base)
-          apply (intro conjI exI)
-           apply (rule refl)
-          apply (rule arg_cong[where f=id_op])
-          apply (rule ext)
-          apply simp
-          apply metis
-          done
-        subgoal for p x buf1' buf2' buf3'
-          apply hypsubst_thin
-          apply simp
-          apply (intro conjI exI)
-           apply (subst id_op_code)
-           apply (rule SC[rotated])
-            apply (rule SW)
-           apply (rule cinsertI2)
-           apply simp
-           apply (rule disjI2)
-           apply (rule image_eqI)
-            apply force
-           apply (simp add: cUNIV.rep_eq)
-          apply (rule bc_base)
-          apply (intro conjI exI)
-           apply (rule refl)
-          apply (rule arg_cong[where f=id_op])
-          apply (rule ext)
-          apply simp
-          done
-        subgoal
-          apply hypsubst_thin
-          apply (intro conjI exI)
-           apply (subst id_op_code)
-           apply (rule SC[rotated])
-            apply simp
-            apply (rule ST)
-           apply simp
-           apply (rule disjI1)
-           apply (rule refl)
-          apply (rule bc_base)
-          apply force
-          done
-        subgoal for p buf1' buf2' buf3'
-          apply hypsubst_thin
-          apply (intro conjI exI)
-           apply (subst id_op_code)
-           apply (rule SC[rotated])
-            apply simp
-            apply (rule ST)
-           apply simp
-           apply (rule disjI1)
-           apply (rule refl)
-          apply (rule bc_base)
-          apply (intro conjI exI)
-           apply (rule refl)
-          apply (rule arg_cong[where f=id_op])
-          apply (rule ext)
-          apply simp
-          done
-        subgoal for p buf1' buf2' buf3'
-          apply hypsubst_thin
-          apply (intro conjI exI)
-           apply (subst id_op_code)
-           apply (rule SC[rotated])
-            apply simp
-            apply (rule ST)
-           apply simp
-           apply (rule disjI1)
-           apply (rule refl)
-          apply (rule bc_base)
-          apply (intro conjI exI)
-           apply (rule refl)
-          apply (rule arg_cong[where f=id_op])
-          apply (rule ext)
-          apply simp
-          done
-        done
-      done
-    subgoal for io op1'
-      apply (cases io)
-      subgoal for p x
-        apply hypsubst_thin
-        apply (drule step_id_op_Inp)
-         apply simp
-        apply hypsubst_thin
-        apply (rule exI[of _ "map_op projl projr (comp_op Some buf2 (id_op (BENQ p x buf1)) (id_op buf3))"])
-        apply (intro conjI)
-        subgoal
-          apply (rule step_map_op[where f=projl and g=projr and io="Inp (Inl p) x", simplified])
-           apply (subst comp_op_code)
-           apply simp
-           apply (rule SC)
-            apply (simp add: Set.filter_def)
-            apply (rule disjI2)
-            apply simp
-            apply (rule disjI1)
-            apply (rule image_eqI)
-             apply (rule refl)
-            apply simp
-            apply (rule disjI1)
-            apply (intro exI)
-            apply (rule refl)
-           apply simp_all
-          apply (rule SR)
-          done
-        subgoal
-          apply (rule bc_sym)
-          apply (rule bc_base)
-          apply (intro conjI exI)
-           apply simp_all
-          apply (rule arg_cong[where f=id_op])
-          apply auto
-          done
-        done
-      subgoal for p x
-        apply hypsubst_thin
-        apply (drule step_id_op_Out)
-         apply simp
-        apply (elim conjE)
-        apply (drule BHD_BAPPEND_2_cases)
-         apply simp
-        apply hypsubst_thin
-        apply (elim exE disjE conjE)
-        subgoal
-          apply (rule exI[of _ "map_op projl projr (comp_op Some buf2 (id_op buf1) (id_op (BTL p buf3)))"])
-          apply (intro conjI)
-          subgoal
-            apply (rule step_map_op[where f=projl and g=projr and io="Out (Inr p) x", simplified])
-             apply (subst comp_op_code)
-             apply simp
-             apply (rule SC)
-              apply (simp add: Set.filter_def)
-              apply (rule disjI2)
-              apply simp
-              apply (rule disjI2)
-              apply (rule image_eqI)
-               apply (rule refl)
-              apply (simp add: cUNIV.rep_eq)
-              apply (intro conjI)
-               apply (rule disjI2)
-               apply (rule disjI2)
-               apply (intro conjI exI)
-                apply assumption
-               apply (rule refl)
-              apply (auto simp add: step.intros(2))
-            done
-          subgoal
-            apply (rule bc_sym)
-            apply (rule bc_base)
-            apply (intro exI conjI) 
-             apply (rule refl)
-            apply (rule arg_cong[where f=id_op])
-            apply (rule ext)
-            apply (auto simp only: split: if_splits)
-              apply (smt (verit, best) fun_upd_apply tl_append2)+
-            done
-          done
-        subgoal
-          apply (rule exI[of _ "map_op projl projr (comp_op Some (BTL p buf2) (id_op buf1) (id_op buf3))"])
-          apply (intro conjI)
-          subgoal
-            apply (rule step_map_op[where f=projl and g=projr and io="Out (Inr p) x", simplified])
-            apply (subst comp_op_code)
-            apply simp
-            apply (rule SC)
-             apply simp
-             apply (rule disjI2)+
-             apply (rule image_eqI)
-              apply (rule refl)
-             apply (simp add: Set.filter_def cUNIV.rep_eq)
-              apply (intro conjI)
-               apply (rule disjI2)
-               apply (rule disjI1)
-            apply (intro conjI exI)
-               apply simp_all
-             apply force
-            apply simp
-           
-
-
-end
-      apply (drule step_comp_op_Some_id_op_id_op)
-        apply simp_all
-      apply (elim exE disjE)
-      subgoal for io' op'' p x
-        apply simp
-        apply (intro conjI exI)
-         apply (subst id_op_code)
-         apply (rule step.intros(3))
-          apply simp
-          apply (rule disjI1)
-          apply (rule image_eqI[of _ _ p])
-           apply (rule refl)
-          apply (simp add: cUNIV.rep_eq)
-         apply (rule step.intros(1))
-        apply (rule bc_base)
-        apply auto
-        apply (intro conjI exI)
-         apply (rule refl)
-        apply (rule arg_cong[where f=id_op]) 
-        apply (auto split: option.splits)
-        apply hypsubst_thin
-        apply (rule ext)
-        apply (clarsimp split: if_splits)
-        apply meson
-        done
-      subgoal for io' op'' p x
-        apply auto
-        subgoal for p'
-          apply (drule sym[of x])
-          apply simp
-          apply hypsubst_thin
-          apply (intro conjI exI)
-           apply (subst id_op_code)
-           apply (rule step.intros(3))
-            apply simp
-            apply (rule disjI2)
-            apply (rule image_eqI[of _ _ p])
-             apply (rule refl)
-            apply (simp add: cUNIV.rep_eq)
-          using step.intros(2) apply force
-          apply (rule bc_base)
-          apply (intro conjI exI)
-           apply (rule refl)
-          apply (rule arg_cong[where f=id_op]) 
-          apply (auto split: option.splits)
-          done
-        done
-      done      
-    subgoal for io op
-      apply (cases io)
-      subgoal for p x
-        apply hypsubst_thin
-        apply (drule step_id_op_Inp)
-         apply simp
-        apply hypsubst_thin
-        apply (rule exI[of _ "map_op projl projr (comp_op Some buf2 (id_op (BENQ p x buf1)) (id_op buf3))"])
-        apply (intro conjI)
-        subgoal
-          apply (rule step_map_op[where f=projl and g=projr and io="Inp (Inl p) x", simplified])
-          apply (subst comp_op_code)
-          apply simp
-          apply (rule step.intros(3))
-           apply (simp add: Set.filter_def)
-           apply (rule disjI1)
-           apply simp
-           apply (rule image_eqI)
-            apply (rule refl)
-           apply simp
-           apply (rule disjI1)
-           apply (rule image_eqI[of _ _ p])
-            apply (rule refl)
-           apply (simp add: cUNIV.rep_eq)
-          apply simp
-          apply (rule step.intros(1))
-          done
-        subgoal
-          apply (rule bc_sym)
-          apply (rule bc_base)
-          apply (intro conjI exI)
-           apply (rule refl)
-          apply (rule arg_cong[where f=id_op])
-          apply (rule ext)
-          apply auto
-          done
-        done
-      subgoal for p x
-        apply hypsubst_thin
-        apply (drule step_id_op_Out)
-         apply simp
-        apply (elim conjE)
-        apply (drule BHD_BAPPEND_2_cases)
-         apply simp
-        apply hypsubst_thin
-        apply (elim exE disjE)
-        subgoal
-          apply (rule exI[of _ "map_op projl projr (comp_op Some buf2 (id_op buf1) (id_op (BTL p buf3)))"])
-          apply (intro conjI)
-          subgoal
-            apply (rule step_map_op[where f=projl and g=projr and io="Out (Inr p) x", simplified])
-            apply (subst comp_op_code)
-            apply simp
-            apply (rule step.intros(3))
-             apply (simp add: Set.filter_def)
-             apply (rule disjI2)
-             apply (rule image_eqI)
-              apply (rule refl)
-             apply (simp add: cUNIV.rep_eq)
-             apply (intro conjI)
-              apply (rule disjI2)
-              apply (rule image_eqI[of _ _ p])
-               apply (rule refl)
-              apply (auto simp add: step.intros(2))
-            done
-          subgoal
-            apply (rule bc_sym)
-            apply (rule bc_base)
-            apply (intro exI conjI) 
-             apply (rule refl)
-            apply (rule arg_cong[where f=id_op])
-            apply (rule ext)
-            apply (auto simp only: split: if_splits)
-              apply (smt (verit, best) fun_upd_apply tl_append2)+
-            done
-          done
-        subgoal
-          apply (rule exI[of _ "map_op projl projr (comp_op Some (BTL p buf2) (id_op buf1) (id_op buf3))"])
-          apply (intro conjI)
-          subgoal
-            apply (rule step_map_op[where f=projl and g=projr and io="Out (Inr p) x", simplified])
-            apply (subst comp_op_code)
-            apply simp
-            apply (rule step.intros(3))
-             apply (simp add: Set.filter_def)
-             apply (rule disjI2)+
-             apply (rule image_eqI)
-              apply (rule refl)
-             apply (simp add: cUNIV.rep_eq)
-             apply (intro conjI)
-              apply (rule disjI1)
-              apply (rule image_eqI[of _ _ p])
-               apply (rule refl)
-              apply simp
-             apply simp
-            apply simp
-            apply (simp add: ranI)
-            apply (subst comp_op_code)
-            apply simp
-            apply (rule step.intros(3))
-             apply (simp add: Set.filter_def)
-             apply (rule disjI2)+
-             apply (rule image_eqI)
-              apply (rule refl)
-             apply (simp add: cUNIV.rep_eq)
-             apply (intro conjI)
-              apply (rule disjI2)
-              apply (rule image_eqI[of _ _ p])
-               apply (rule refl)
-              apply simp_all
-            apply (metis fun_upd_triv step.intros(2))
-            done
-          subgoal
-            apply (rule bc_sym)
-            apply (rule bc_base)
-            apply (intro exI conjI) 
-             apply (rule refl)
-            apply (rule arg_cong[where f=id_op])
-            apply (rule ext)
-            apply (auto simp only:  split: if_splits)
-             apply (smt (verit, best) append_self_conv2 fun_upd_other fun_upd_same tl_append2)+
-            done
-          done
-        subgoal
-          apply (elim conjE)
-          apply (rule exI[of _ "map_op projl projr (comp_op Some buf2 (id_op (BTL p buf1)) (id_op buf3))"])
-          apply (intro conjI)
-          subgoal
-            apply (rule step_map_op[where f=projl and g=projr and io="Out (Inr p) x", simplified])
-            apply (subst (1) comp_op_code)
-            apply simp
-            apply (rule step.intros(3))
-             apply (simp add: cUNIV.rep_eq Set.filter_def)
-             apply (rule disjI1)
-             apply simp
-             apply (rule image_eqI)
-              defer
-              apply (simp add: cUNIV.rep_eq)
-              apply (rule disjI2)
-              apply (rule image_eqI[of _ _ p])
-               apply (rule refl)
-              apply simp
-             apply simp_all
-            apply (subst (1) comp_op_code)
-            apply (rule step.intros(3))
-             apply (simp add: cUNIV.rep_eq Set.filter_def)
-             apply (rule disjI2)
-             apply (rule image_eqI)
-              apply (rule refl)
-             apply simp_all
-             apply (intro conjI)
-              apply (rule disjI1)
-              apply (rule image_eqI[of _ _ p])
-               apply (rule refl)
-              apply (simp_all add: ranI)
-            apply (subst (1) comp_op_code)
-            apply (rule step.intros(3))
-             apply simp
-             apply (rule disjI2)
-             apply (rule image_eqI)
-              apply (rule refl)
-             apply simp
-             apply (intro conjI)
-              apply (rule disjI2)
-              apply (rule image_eqI[of _ _ p])
-               apply (rule refl)
-              apply simp
-            using cUNIV.rep_eq apply blast
-             apply simp_all
-            apply (metis fun_upd_triv step.simps)
-            done
-          subgoal
-            apply (rule bc_sym)
-            apply (rule bc_base)
-            apply (intro exI conjI) 
-             apply (rule refl)
-            apply (rule arg_cong[where f=id_op])
-            apply (rule ext)
-            apply (auto simp only:  split: if_splits)
-            apply (smt (verit, best) append_self_conv2 fun_upd_other fun_upd_same tl_append2)+
-            done
-          done
-        done
-      done
-    done
-  done
+  done *)
 
 end
